ifc-machine/pico/tmu/cmach/Backward.v
@@ -1,0 +1,84 @@
+Require Import List.
+Require Import ZArith.
+
+Require Import Utils.
+Require Import Lattices.
+Require Import CLattices.
+Require Import WfCLattices.
+Require Import TMUInstr.
+Require Import Abstract.
+Require Import AbstractCommon.
+Require Import Rules.
+Require Import QuasiAbstractMachine.
+Require Import Concrete.
+Require Import ConcreteMachineSmallStep.
+Require Import Determinism.
+Require Import Refinement.
+Require Import CExec.
+Require Import BackwardCacheMiss.
+Require Import BackwardCacheHit.
+Require Import Ref.
+
+Open Scope Z_scope.
+
+Set Implicit Arguments.
+
+Section Backward.
+
+Context {L: Type}
+        {Latt: JoinSemiLattice L}
+        {CLatt: ConcreteLattice L}
+        {WFCLatt: WfConcreteLattice L Latt CLatt}.
+
+Definition match_events e1 e2 :=
+  e1 = abstract_event e2.
+
+Definition remove_none {T} (l : list (option T)) :=
+  filter (@is_some _) l.
+
+Lemma filter_cons_inv :
+  forall A (f : A -> bool) a l1 l2,
+    a :: l1 = filter f l2 ->
+    exists l2', l1 = filter f l2'.
+Proof.
+  induction l2 as [|a' l2 IH]; simpl. congruence.
+  destruct (f a'); intros H; auto.
+  inv H. eauto.
+Qed.
+
+Lemma backward_simulation_pre_obs :
+  backward_simulation step_rules cstep match_states match_events
+                      remove_none remove_none.
+Proof.
+  intros s1 s2 t2 s2' MATCH EXEC.
+  apply exec_cexec in EXEC.
+  match type of EXEC with
+    | cexec _ ?T _ =>
+      remember T as t2'
+  end.
+  gdep t2. gdep s1.
+  unfold remove_none.
+  induction EXEC; intros s1 MATCH t2 Ht2; unfold remove_none.
+  - exists nil. exists s1.
+    split. constructor.
+    rewrite <- Ht2. constructor.
+  - inv MATCH.
+    apply kernel_run_until_user_l in H.
+    inv H.
+  - exploit cache_hit_simulation; eauto.
+    intros [s1' [STEP MATCH']].
+    assert (exists t', t = filter (@is_some _) t') by
+        (destruct e; eauto using filter_cons_inv).
+    inv H2.
+    exploit IHEXEC; eauto.
+    intros [? [? [? ?]]].
+    eexists. eexists.
+    split. econstructor 2; eauto.
+    rewrite <- Ht2.
+    destruct e as [[[? ?]]|]; simpl; eauto.
+    constructor; auto.
+    reflexivity.
+  - exploit cache_miss_simulation; eauto.
+Qed.
+
+End Backward.
